document llft logic

src/guarding/lib/lifetime.v
@@ -15,6 +15,8 @@ From iris.proofmode Require Import tactics.
 From iris.proofmode Require Import coq_tactics.
 From iris.base_logic.lib Require Export invariants.
 
+(** Leaf Lifetime Logic. Based loosely on RustBelt's lifetime logic. *)
+
 (* begin hide *)
 
 Inductive LtRa :=
@@ -137,675 +139,712 @@ Proof.
   solve_inG.
 Qed.
 
-Section LtResource.
+Section LlftLogic.
 
-Context {Σ: gFunctors}.
-Context `{!lt_logicG Σ}.
-Context `{!invGS Σ}.
+  Context {Σ: gFunctors}.
+  Context `{!lt_logicG Σ}.
+  Context `{!invGS Σ}.
 
-Context (γlt : gname).
+  Context (γlt : gname).
 
-(* begin hide *)
+  (* begin hide *)
 
-Definition lt_state (sa sd : gset nat) := LtOk (Some (sa, sd)) ∅ sd.
-Definition LtState (sa sd : gset nat) : iProp Σ := own γlt (lt_state sa sd).
+  Definition lt_state (sa sd : gset nat) := LtOk (Some (sa, sd)) ∅ sd.
+  Definition LtState (sa sd : gset nat) : iProp Σ := own γlt (lt_state sa sd).
 
-Definition dead (k: nat) := LtOk None ∅ ({[ k ]}).
-Definition Dead (k: nat) : iProp Σ := own γlt (dead k).
+  Definition dead (k: nat) := LtOk None ∅ ({[ k ]}).
+  Definition Dead (k: nat) : iProp Σ := own γlt (dead k).
 
-Definition alive (k: nat) := LtOk None ({[+ k +]}) ∅.
-Definition Alive (k: nat) : iProp Σ := own γlt (alive k).
+  Definition alive (k: nat) := LtOk None ({[+ k +]}) ∅.
+  Definition Alive (k: nat) : iProp Σ := own γlt (alive k).
 
-Lemma update_helper (a b : LtRa)
-  (cond: ∀ z : ltR, lt_inv (a ⋅ z) → lt_inv (b ⋅ z))
-  : a ~~> b.
-Proof.
-  rewrite cmra_discrete_total_update.
-  intros y ay. destruct ay as [t ay]. rewrite <- lt_assoc in ay.
-  have co := cond _ ay. exists t. rewrite <- lt_assoc. apply co.
-Qed.
+  Lemma update_helper (a b : LtRa)
+    (cond: ∀ z : ltR, lt_inv (a ⋅ z) → lt_inv (b ⋅ z))
+    : a ~~> b.
+  Proof.
+    rewrite cmra_discrete_total_update.
+    intros y ay. destruct ay as [t ay]. rewrite <- lt_assoc in ay.
+    have co := cond _ ay. exists t. rewrite <- lt_assoc. apply co.
+  Qed.
 
-Lemma update_helper2 (x y : LtRa)
-  (cond: ∀ o a d , lt_inv (x ⋅ LtOk o a d) → lt_inv (y ⋅ LtOk o a d))
-  : x ~~> y.
-Proof.
-  apply update_helper. intros z. destruct z as [o a d|].
-  - apply cond.
-  - intros lti. unfold lt_inv in lti.
-    replace (x ⋅ LtFail) with LtFail in lti. { contradiction. }
-    destruct x as [o a d|]; trivial. destruct o; trivial.
-Qed.
+  Lemma update_helper2 (x y : LtRa)
+    (cond: ∀ o a d , lt_inv (x ⋅ LtOk o a d) → lt_inv (y ⋅ LtOk o a d))
+    : x ~~> y.
+  Proof.
+    apply update_helper. intros z. destruct z as [o a d|].
+    - apply cond.
+    - intros lti. unfold lt_inv in lti.
+      replace (x ⋅ LtFail) with LtFail in lti. { contradiction. }
+      destruct x as [o a d|]; trivial. destruct o; trivial.
+  Qed.
 
-Lemma new_lt k sa sd :
-  (k ∉ sa) → (k ∉ sd) →
-  LtState sa sd ==∗ LtState (sa ∪ {[ k ]}) sd ∗ Alive k ∗ Alive k.
-Proof.
-  intros k_sa k_sd.
-  setoid_rewrite <- own_op. setoid_rewrite <- own_op.
-  iIntros "a". iApply own_update. 2: { iFrame "a". } apply update_helper2.
-  
-  intros o a d lti. destruct o as [s|].
-  - contradiction. (*unfold "⋅", lt_op, lt_state, lt_inv in lti. contradiction.*)
-  - simpl in lti. destruct lti as [sd_d [no_int fm]].
-    simpl. split. { set_solver. }
-    split. { set_solver. }
-    intro m. split. {
-        intro m_in. have fmm := fm m. destruct fmm as [fmm1 fmm2].
-        rewrite elem_of_union in m_in. destruct m_in as [m_in|m_k].
-        + rewrite gmultiset_disj_union_left_id.
+  Lemma new_lt k sa sd :
+    (k ∉ sa) → (k ∉ sd) →
+    LtState sa sd ==∗ LtState (sa ∪ {[ k ]}) sd ∗ Alive k ∗ Alive k.
+  Proof.
+    intros k_sa k_sd.
+    setoid_rewrite <- own_op. setoid_rewrite <- own_op.
+    iIntros "a". iApply own_update. 2: { iFrame "a". } apply update_helper2.
+
+    intros o a d lti. destruct o as [s|].
+    - contradiction. (*unfold "⋅", lt_op, lt_state, lt_inv in lti. contradiction.*)
+    - simpl in lti. destruct lti as [sd_d [no_int fm]].
+      simpl. split. { set_solver. }
+      split. { set_solver. }
+      intro m. split. {
+          intro m_in. have fmm := fm m. destruct fmm as [fmm1 fmm2].
+          rewrite elem_of_union in m_in. destruct m_in as [m_in|m_k].
+          + rewrite gmultiset_disj_union_left_id.
+            rewrite multiplicity_disj_union.
+            have fmm11 := fmm1 m_in.
+            rewrite gmultiset_disj_union_left_id in fmm11. rewrite fmm11.
+            rewrite multiplicity_disj_union.
+            rewrite multiplicity_singleton_ne. { trivial. }
+            intro mk. subst m. apply k_sa. apply m_in.
+          + rewrite gmultiset_disj_union_left_id.
+            rewrite multiplicity_disj_union.
+            rewrite multiplicity_disj_union.
+            rewrite elem_of_singleton in m_k. rewrite m_k.
+            rewrite multiplicity_singleton.
+            have fmk := fm k. destruct fmk as [_ fmk0].
+            rewrite gmultiset_disj_union_left_id in fmk0.
+            rewrite fmk0; trivial.
+          }
+          intros m_not_in. rewrite not_elem_of_union in m_not_in.
+          destruct m_not_in as [m_sa m_k].
+          rewrite gmultiset_disj_union_left_id.
           rewrite multiplicity_disj_union.
-          have fmm11 := fmm1 m_in.
-          rewrite gmultiset_disj_union_left_id in fmm11. rewrite fmm11.
           rewrite multiplicity_disj_union.
-          rewrite multiplicity_singleton_ne. { trivial. }
-          intro mk. subst m. apply k_sa. apply m_in.
-        + rewrite gmultiset_disj_union_left_id.
+          have fmm := fm m. destruct fmm as [_ fmm0]. 
+          rewrite gmultiset_disj_union_left_id in fmm0. rewrite fmm0; trivial.
+          rewrite not_elem_of_singleton in m_k.
+          rewrite multiplicity_singleton_ne; trivial.
+  Qed.
+
+  Lemma double_incl_lt_inv a b z' :
+    (a ≼ z') → (b ≼ z') → (✓ z') → ∃ z, a ≼ z ∧ b ≼ z ∧ lt_inv z.
+  Proof.
+    intros az bz valz. destruct valz as [t valz]. exists (z' ⋅ t).
+    split.
+    { destruct az as [t1 az]. rewrite az. exists (t1 ⋅ t). rewrite <- lt_assoc. trivial. }
+    split.
+    { destruct bz as [t1 bz]. rewrite bz. exists (t1 ⋅ t). rewrite <- lt_assoc. trivial. }
+    trivial.
+  Qed.
+
+  Lemma lt_state_incl_lt_ok sa sd sa1 sd1 a d 
+    : (lt_state sa sd ≼ LtOk (Some (sa1, sd1)) a d) → sa = sa1 ∧ sd = sd1.
+  Proof.
+    intros lts. destruct lts as [t lts].
+    destruct t as [[o|] a1 d1|].
+    - unfold lt_state in lts. unfold "⋅", lt_op in lts. inversion lts.
+    - unfold lt_state in lts. unfold "⋅", lt_op in lts. inversion lts. split; trivial.
+    - unfold lt_state in lts. unfold "⋅", lt_op in lts. inversion lts.
+  Qed.
+
+  Lemma alive_incl_lt_ok k sa1 sd1 a d
+    : (alive k ≼ LtOk (Some (sa1, sd1)) a d) → lt_inv (LtOk (Some (sa1, sd1)) a d) → k ∈ sa1.
+  Proof.
+    intros lts lti. destruct lts as [t lts].
+    destruct t as [[o|] a1 d1|].
+    - unfold alive in lts. unfold "⋅", lt_op in lts. inversion lts.
+        unfold lt_inv in lti. destruct lti as [_ [_ fm]]. have fmk := fm k.
+        have h : Decision (k ∈ sa1) by solve_decision. destruct h as [h|n]; trivial.
+        exfalso.
+        destruct fmk as [_ fmk]. have fmk1 := fmk n. subst a.
+        rewrite multiplicity_disj_union in fmk1.
+        rewrite multiplicity_singleton in fmk1. lia.
+    - inversion lts.
+    - inversion lts.
+  Qed.
+
+  Lemma dead_incl_lt_ok k sa1 sd1 a d
+    : (dead k ≼ LtOk (Some (sa1, sd1)) a d) → lt_inv (LtOk (Some (sa1, sd1)) a d) → k ∈ sd1.
+  Proof.
+    intros lts lti. destruct lts as [t lts].
+    destruct t as [[o|] a1 d1|].
+    - unfold dead in lts. unfold "⋅", lt_op in lts. inversion lts.
+        unfold lt_inv in lti. destruct lti as [sde _]. subst d. set_solver.
+    - inversion lts.
+    - inversion lts.
+  Qed.
+
+  Lemma alive_dead_contradiction k sa sd a d
+    : (lt_inv (LtOk (Some (sa, sd)) a d)) → (k ∈ sa) → (k ∈ sd) → False.
+  Proof.
+    intros lts lti. destruct lts as [_ [no_int _]]. set_solver.
+  Qed.
+
+  Lemma lt_state_alive k sa sd :
+    LtState sa sd ∧ Alive k ⊢ ⌜ k ∈ sa ⌝.
+  Proof.
+    iIntros "P". iDestruct (and_own_discrete_ucmra with "P") as (z') "[o [%incl1 %incl2]]".
+    iDestruct (own_valid with "o") as "%valz".
+    iPureIntro.
+    have di := double_incl_lt_inv _ _ _ incl1 incl2 valz.
+    destruct di as [z [inc1 [inc2 lti]]].
+    destruct z as [[[sa1 sd1]|] a d|]; try contradiction.
+    have j := lt_state_incl_lt_ok _ _ _ _ _ _ inc1. destruct j as [j1 j2]. subst sa.
+    apply (alive_incl_lt_ok _ _ _ _ _ inc2). apply lti.
+  Qed.
+
+  Lemma lt_state_dead k sa sd :
+    LtState sa sd ∧ Dead k ⊢ ⌜ k ∈ sd ⌝.
+  Proof.
+    iIntros "P". iDestruct (and_own_discrete_ucmra with "P") as (z') "[o [%incl1 %incl2]]".
+    iDestruct (own_valid with "o") as "%valz".
+    iPureIntro.
+    have di := double_incl_lt_inv _ _ _ incl1 incl2 valz.
+    destruct di as [z [inc1 [inc2 lti]]].
+    destruct z as [[[sa1 sd1]|] a d|]; try contradiction.
+    have j := lt_state_incl_lt_ok _ _ _ _ _ _ inc1. destruct j as [j1 j2]. subst sd.
+    apply (dead_incl_lt_ok _ _ _ _ _ inc2). apply lti.
+  Qed.
+
+  Lemma lt_alive_dead_false k :
+    Alive k ∧ Dead k ⊢ False.
+  Proof.
+    iIntros "P". iDestruct (and_own_discrete_ucmra with "P") as (z') "[o [%incl1 %incl2]]".
+    iDestruct (own_valid with "o") as "%valz".
+    iPureIntro.
+    have di := double_incl_lt_inv _ _ _ incl1 incl2 valz.
+    destruct di as [z [inc1 [inc2 lti]]].
+    destruct z as [[[sa1 sd1]|] a d|]; try contradiction.
+    have j1 := alive_incl_lt_ok _ _ _ _ _ inc1.
+    have j2 := dead_incl_lt_ok _ _ _ _ _ inc2.
+    eapply alive_dead_contradiction. { apply lti. } { apply j1. apply lti. } { apply j2. apply lti. }
+  Qed.
+
+  Lemma kill_lt k sa sd :
+    LtState sa sd ∗ Alive k ∗ Alive k ==∗ LtState (sa ∖ {[ k ]}) (sd ∪ {[ k ]}) ∗ Dead k.
+  Proof.
+    setoid_rewrite <- own_op. setoid_rewrite <- own_op.
+    iIntros "a". iApply own_update. 2: { iFrame "a". } apply update_helper2.
+
+    intros o a d lti. destruct o as [s|].
+    - contradiction.
+    - simpl in lti. destruct lti as [sd_d [no_int fm]].
+      simpl. split. { set_solver. }
+      split. { set_solver. }
+      intro m. split. {
+          intro m_in. have fmm := fm m. destruct fmm as [fmm1 fmm2].
+          rewrite gmultiset_disj_union_left_id.
+          rewrite gmultiset_disj_union_left_id.
+          rewrite gmultiset_disj_union_left_id in fmm1.
+          rewrite multiplicity_disj_union in fmm1.
+          rewrite multiplicity_disj_union in fmm1.
+          rewrite elem_of_difference in m_in. destruct m_in as [m_in mk].
+          rewrite elem_of_singleton in mk.
+          rewrite multiplicity_singleton_ne in fmm1; trivial.
+          apply fmm1. apply m_in.
+      }
+          intro m_in. have fmm := fm m. destruct fmm as [fmm1 fmm2].
+          rewrite gmultiset_disj_union_left_id.
+          rewrite gmultiset_disj_union_left_id.
+          rewrite gmultiset_disj_union_left_id in fmm2.
+          rewrite multiplicity_disj_union in fmm1.
+          rewrite multiplicity_disj_union in fmm1.
+          rewrite not_elem_of_difference in m_in.
+          have h : Decision (m ∈ sa) by solve_decision. destruct h as [h|n].
+          + destruct m_in as [m_not_in_sa|mk].
+            * exfalso. apply m_not_in_sa. apply h.
+            * rewrite multiplicity_disj_union in fmm1.
+              have fmm1i := fmm1 h.
+              rewrite elem_of_singleton in mk. subst m. rewrite multiplicity_singleton in fmm1i.
+                rewrite multiplicity_empty in fmm1i. lia.
+          + have fmm2i := fmm2 n.
+            rewrite multiplicity_disj_union in fmm2i.
+            rewrite multiplicity_disj_union in fmm2i. lia.
+  Qed.
+
+  Lemma bigSepS_alive_equiv_own a
+    (ne_emp: a ≠ ∅)
+      : ([∗ set] k ∈ a, Alive k) ⊣⊢ own γlt (LtOk None (list_to_set_disj (elements a)) ∅).
+  Proof.
+    induction a as [|x T ? IH] using set_ind_L. 
+    - contradiction.
+    - have h : Decision (T = ∅) by solve_decision. destruct h as [h|n]; trivial.
+      + subst T. rewrite big_sepS_union; last by set_solver.
+        rewrite big_sepS_empty. rewrite big_sepS_singleton. unfold Alive, alive.
+        rewrite union_empty_r. rewrite elements_singleton. unfold list_to_set_disj.
+        rewrite bi.sep_emp. rewrite gmultiset_disj_union_right_id. trivial.
+      + rewrite big_sepS_union; last by set_solver.
+        rewrite (IH n). rewrite big_sepS_singleton. unfold Alive, alive.
+          rewrite <- own_op.
+          f_equiv.
+          unfold "⋅", cmra_op, ltR, lt_op. f_equiv; last by set_solver.
+          rewrite elements_union_singleton; trivial.
+  Qed.
+
+  Lemma lt_ok_none_left o a1 d1 a2 d2
+      : LtOk None a1 d1 ⋅ LtOk o a2 d2 = LtOk o (a1 ⊎ a2) (d1 ∪ d2).
+  Proof.
+    destruct o as [o|]; trivial.
+  Qed.
+
+  Lemma mult_list_to_set_disj_not_in (a: gset nat) (x: nat)
+    (not_in: x ∉ a) : multiplicity x (list_to_set_disj (elements a)) = 0.
+  Proof.
+  induction a as [|y b ? IH] using set_ind_L. 
+  - trivial.
+  - rewrite elements_union_singleton; trivial. rewrite list_to_set_disj_cons.
+      rewrite multiplicity_disj_union. rewrite IH; last by set_solver.
+      assert (x ≠ y) by set_solver. rewrite multiplicity_singleton_ne; trivial.
+  Qed.
+
+  Lemma mult_list_to_set_disj_in (a: gset nat) (x: nat)
+    (is_in: x ∈ a) : multiplicity x (list_to_set_disj (elements a)) = 1.
+  Proof.
+  induction a as [|y b ? IH] using set_ind_L. 
+  - rewrite elem_of_empty in is_in. contradiction.
+  - rewrite elements_union_singleton; trivial. rewrite list_to_set_disj_cons.
+      rewrite multiplicity_disj_union.
+      rewrite elem_of_union in is_in. destruct is_in as [ix|ib].
+      + rewrite elem_of_singleton in ix. subst x. rewrite mult_list_to_set_disj_not_in; trivial.
+          rewrite multiplicity_singleton. trivial.
+      + rewrite (IH ib). rewrite multiplicity_singleton_ne; trivial. intro x_eq_y.
+          subst x. contradiction.
+  Qed.
+
+  Lemma multiplicity_le o1 a1 d1 o2 a2 d2 x
+    : LtOk o1 a1 d1 ≼ LtOk o2 a2 d2 → multiplicity x a1 ≤ multiplicity x a2.
+  Proof.
+    intro incl. destruct incl as [t incl]. destruct t as [o3 a3 d3|].
+    - assert (a2 = a1 ⊎ a3) as X.
+        + unfold "⋅", lt_op in incl. destruct o1; destruct o3.
+          * inversion incl. * inversion incl; trivial. * inversion incl; trivial.
+          * inversion incl; trivial.
+        + subst a2. rewrite multiplicity_disj_union. lia.
+    - unfold "⋅", lt_op in incl. destruct o1; inversion incl.
+  Qed.
+
+  Lemma own_and_alive (a1 a2 : gset nat)
+    : own γlt (LtOk None (list_to_set_disj (elements a1)) ∅)
+      ∧ own γlt (LtOk None (list_to_set_disj (elements a2)) ∅)
+      ⊢ own γlt (LtOk None (list_to_set_disj (elements (a1 ∪ a2))) ∅).
+  Proof.
+    iIntros "x".
+    iDestruct (and_own_discrete_ucmra_specific with "x") as "y"; last by iFrame "y".
+    intros w valw incl1 incl2.
+    destruct w as [o a d|].
+    - exists (LtOk o (a ∖ (list_to_set_disj (elements (a1 ∪ a2)))) d).
+      rewrite lt_ok_none_left. f_equiv.
+      + rewrite gmultiset_eq. intros x.
           rewrite multiplicity_disj_union.
-          rewrite multiplicity_disj_union.
-          rewrite elem_of_singleton in m_k. rewrite m_k.
-          rewrite multiplicity_singleton.
-          have fmk := fm k. destruct fmk as [_ fmk0].
-          rewrite gmultiset_disj_union_left_id in fmk0.
-          rewrite fmk0; trivial.
-        }
-        intros m_not_in. rewrite not_elem_of_union in m_not_in.
-        destruct m_not_in as [m_sa m_k].
-        rewrite gmultiset_disj_union_left_id.
-        rewrite multiplicity_disj_union.
-        rewrite multiplicity_disj_union.
-        have fmm := fm m. destruct fmm as [_ fmm0]. 
-        rewrite gmultiset_disj_union_left_id in fmm0. rewrite fmm0; trivial.
-        rewrite not_elem_of_singleton in m_k.
-        rewrite multiplicity_singleton_ne; trivial.
-Qed.
+          rewrite multiplicity_difference.
+          enough ((multiplicity x a ≥ multiplicity x (list_to_set_disj (elements (a1 ∪ a2))))).
+          { lia. }
+          have t1 := multiplicity_le _ _ _ _ _ _ x incl1.
+          have t2 := multiplicity_le _ _ _ _ _ _ x incl2.
+          have h : Decision (x ∈ a1) by solve_decision. destruct h as [h1|n1]; trivial.
+            *  rewrite mult_list_to_set_disj_in in t1; trivial.
+              rewrite mult_list_to_set_disj_in; last by set_solver.
+              lia.
+          * have q : Decision (x ∈ a2) by solve_decision. destruct q as [h2|n2]; trivial.
+            -- rewrite mult_list_to_set_disj_in in t2; trivial.
+              rewrite mult_list_to_set_disj_in; last by set_solver.
+              lia.
+            -- rewrite mult_list_to_set_disj_not_in; last by set_solver.
+              lia.
+      + set_solver.
+    - unfold "✓", cmra_valid, ucmra_cmraR, ucmra_valid, ltUR, lt_valid in valw.
+      destruct valw as [b valw].
+      replace (LtFail ⋅ b) with LtFail in valw. { contradiction. }
+      destruct b; trivial.
+  Qed.
 
-Lemma double_incl_lt_inv a b z' :
-  (a ≼ z') → (b ≼ z') → (✓ z') → ∃ z, a ≼ z ∧ b ≼ z ∧ lt_inv z.
-Proof.
-  intros az bz valz. destruct valz as [t valz]. exists (z' ⋅ t).
-  split.
-  { destruct az as [t1 az]. rewrite az. exists (t1 ⋅ t). rewrite <- lt_assoc. trivial. }
-  split.
-  { destruct bz as [t1 bz]. rewrite bz. exists (t1 ⋅ t). rewrite <- lt_assoc. trivial. }
-  trivial.
-Qed.
+  Lemma alive_and_bigSepS (a1 a2 : gset nat)
+    : ([∗ set] k ∈ a1, Alive k) ∧ ([∗ set] k ∈ a2, Alive k)
+      ⊢ [∗ set] k ∈ a1 ∪ a2, Alive k.
+  Proof.
+    have h: Decision (a1 = ∅) by solve_decision. destruct h as [h1|n1].
+    { subst a1. rewrite big_sepS_empty. rewrite bi.emp_and.
+        rewrite big_sepS_union; last by set_solver.
+        rewrite big_sepS_empty. rewrite bi.emp_sep. trivial. }
+    have h: Decision (a2 = ∅) by solve_decision. destruct h as [h2|n2].
+    { subst a2. rewrite big_sepS_empty. rewrite bi.and_emp.
+        rewrite big_sepS_union; last by set_solver.
+        rewrite big_sepS_empty. rewrite bi.sep_emp. trivial. }
+    rewrite bigSepS_alive_equiv_own; trivial.
+    rewrite bigSepS_alive_equiv_own; trivial.
+    rewrite bigSepS_alive_equiv_own; last by set_solver.
+    apply own_and_alive.
+  Qed.
 
-Lemma lt_state_incl_lt_ok sa sd sa1 sd1 a d 
-  : (lt_state sa sd ≼ LtOk (Some (sa1, sd1)) a d) → sa = sa1 ∧ sd = sd1.
-Proof.
-  intros lts. destruct lts as [t lts].
-  destruct t as [[o|] a1 d1|].
-  - unfold lt_state in lts. unfold "⋅", lt_op in lts. inversion lts.
-  - unfold lt_state in lts. unfold "⋅", lt_op in lts. inversion lts. split; trivial.
-  - unfold lt_state in lts. unfold "⋅", lt_op in lts. inversion lts.
-Qed.
-  
-Lemma alive_incl_lt_ok k sa1 sd1 a d
-  : (alive k ≼ LtOk (Some (sa1, sd1)) a d) → lt_inv (LtOk (Some (sa1, sd1)) a d) → k ∈ sa1.
-Proof.
-  intros lts lti. destruct lts as [t lts].
-  destruct t as [[o|] a1 d1|].
-  - unfold alive in lts. unfold "⋅", lt_op in lts. inversion lts.
-      unfold lt_inv in lti. destruct lti as [_ [_ fm]]. have fmk := fm k.
-      have h : Decision (k ∈ sa1) by solve_decision. destruct h as [h|n]; trivial.
-      exfalso.
-      destruct fmk as [_ fmk]. have fmk1 := fmk n. subst a.
-      rewrite multiplicity_disj_union in fmk1.
-      rewrite multiplicity_singleton in fmk1. lia.
-  - inversion lts.
-  - inversion lts.
-Qed.
-  
-Lemma dead_incl_lt_ok k sa1 sd1 a d
-  : (dead k ≼ LtOk (Some (sa1, sd1)) a d) → lt_inv (LtOk (Some (sa1, sd1)) a d) → k ∈ sd1.
-Proof.
-  intros lts lti. destruct lts as [t lts].
-  destruct t as [[o|] a1 d1|].
-  - unfold dead in lts. unfold "⋅", lt_op in lts. inversion lts.
-      unfold lt_inv in lti. destruct lti as [sde _]. subst d. set_solver.
-  - inversion lts.
-  - inversion lts.
-Qed.
-  
-Lemma alive_dead_contradiction k sa sd a d
-  : (lt_inv (LtOk (Some (sa, sd)) a d)) → (k ∈ sa) → (k ∈ sd) → False.
-Proof.
-  intros lts lti. destruct lts as [_ [no_int _]]. set_solver.
-Qed.
+  Local Instance pers_dead k : Persistent (Dead k).
+  Proof.
+    apply own_core_persistent. unfold CoreId. trivial.
+  Qed.
 
-Lemma lt_state_alive k sa sd :
-  LtState sa sd ∧ Alive k ⊢ ⌜ k ∈ sa ⌝.
-Proof.
-  iIntros "P". iDestruct (and_own_discrete_ucmra with "P") as (z') "[o [%incl1 %incl2]]".
-  iDestruct (own_valid with "o") as "%valz".
-  iPureIntro.
-  have di := double_incl_lt_inv _ _ _ incl1 incl2 valz.
-  destruct di as [z [inc1 [inc2 lti]]].
-  destruct z as [[[sa1 sd1]|] a d|]; try contradiction.
-  have j := lt_state_incl_lt_ok _ _ _ _ _ _ inc1. destruct j as [j1 j2]. subst sa.
-  apply (alive_incl_lt_ok _ _ _ _ _ inc2). apply lti.
-Qed.
+  Lemma LtState_entails_Dead k sa sd : (k ∈ sd) → LtState sa sd ⊢ Dead k.
+  Proof.
+    intros ksd.
+    unfold LtState.
+    replace (lt_state sa sd) with (lt_state sa sd ⋅ dead k).
+    { rewrite own_op. iIntros "[A B]". iFrame "B". }
+    unfold dead, lt_state, "⋅", lt_op. f_equal. set_solver.
+  Qed.
 
-Lemma lt_state_dead k sa sd :
-  LtState sa sd ∧ Dead k ⊢ ⌜ k ∈ sd ⌝.
-Proof.
-  iIntros "P". iDestruct (and_own_discrete_ucmra with "P") as (z') "[o [%incl1 %incl2]]".
-  iDestruct (own_valid with "o") as "%valz".
-  iPureIntro.
-  have di := double_incl_lt_inv _ _ _ incl1 incl2 valz.
-  destruct di as [z [inc1 [inc2 lti]]].
-  destruct z as [[[sa1 sd1]|] a d|]; try contradiction.
-  have j := lt_state_incl_lt_ok _ _ _ _ _ _ inc1. destruct j as [j1 j2]. subst sd.
-  apply (dead_incl_lt_ok _ _ _ _ _ inc2). apply lti.
-Qed.
+  Lemma LtState_disjoint sa sd : LtState sa sd ⊢ ⌜ sa ∩ sd = ∅ ⌝.
+  Proof.
+    iIntros "T". iDestruct (own_valid with "T") as "%val". iPureIntro.
+    destruct val as [t lts].
+    destruct t as [[o|] a d|].
+    - inversion lts.
+    - simpl in lts. intuition.
+    - inversion lts.
+  Qed.
 
-Lemma lt_alive_dead_false k :
-  Alive k ∧ Dead k ⊢ False.
-Proof.
-  iIntros "P". iDestruct (and_own_discrete_ucmra with "P") as (z') "[o [%incl1 %incl2]]".
-  iDestruct (own_valid with "o") as "%valz".
-  iPureIntro.
-  have di := double_incl_lt_inv _ _ _ incl1 incl2 valz.
-  destruct di as [z [inc1 [inc2 lti]]].
-  destruct z as [[[sa1 sd1]|] a d|]; try contradiction.
-  have j1 := alive_incl_lt_ok _ _ _ _ _ inc1.
-  have j2 := dead_incl_lt_ok _ _ _ _ _ inc2.
-  eapply alive_dead_contradiction. { apply lti. } { apply j1. apply lti. } { apply j2. apply lti. }
-Qed.
+  Definition Cancel (γ: gname) : iProp Σ := own γ (Excl ()).
+  Lemma new_cancel : ⊢ |==> ∃ γ , Cancel γ.
+  Proof.
+    iIntros. iDestruct (own_alloc (Excl ())) as "H"; first done. unfold Cancel. iFrame "H".
+  Qed.
+  Local Lemma cancel_cancel_false (γc : gname) : Cancel γc ∗ Cancel γc ⊢ False.
+  Proof.
+    iIntros "X". unfold Cancel. rewrite <- own_op.
+    iDestruct (own_valid with "X") as "%J". contradiction.
+  Qed.
 
-Lemma kill_lt k sa sd :
-  LtState sa sd ∗ Alive k ∗ Alive k ==∗ LtState (sa ∖ {[ k ]}) (sd ∪ {[ k ]}) ∗ Dead k.
-Proof.
-  setoid_rewrite <- own_op. setoid_rewrite <- own_op.
-  iIntros "a". iApply own_update. 2: { iFrame "a". } apply update_helper2.
-  
-  intros o a d lti. destruct o as [s|].
-  - contradiction.
-  - simpl in lti. destruct lti as [sd_d [no_int fm]].
-    simpl. split. { set_solver. }
-    split. { set_solver. }
-    intro m. split. {
-        intro m_in. have fmm := fm m. destruct fmm as [fmm1 fmm2].
-        rewrite gmultiset_disj_union_left_id.
-        rewrite gmultiset_disj_union_left_id.
-        rewrite gmultiset_disj_union_left_id in fmm1.
-        rewrite multiplicity_disj_union in fmm1.
-        rewrite multiplicity_disj_union in fmm1.
-        rewrite elem_of_difference in m_in. destruct m_in as [m_in mk].
-        rewrite elem_of_singleton in mk.
-        rewrite multiplicity_singleton_ne in fmm1; trivial.
-        apply fmm1. apply m_in.
+  Local Lemma not_subset_eq_get (a b : gset nat) : (a ⊈ b) → ∃ k , k ∈ a ∧ k ∉ b.
+  Proof.
+    assert (∀ r , list_to_set r ⊈ b → ∃ u: nat , u ∈ ((list_to_set r) : gset nat) ∧ u ∉ b) as X.
+    { intro r. induction r as [|a0 r IHr].
+      - intros emp. rewrite list_to_set_nil in emp. set_solver.
+      - intros not_in. rewrite list_to_set_cons in not_in.
+        destruct (decide (a0 ∈ b)); trivial.
+        + assert (list_to_set r ⊈ b) as K by set_solver.
+          have IHr2 := IHr K. destruct IHr2 as [u IHr2]. exists u. set_solver.
+        + exists a0. intuition. rewrite list_to_set_cons. set_solver.
     }
-        intro m_in. have fmm := fm m. destruct fmm as [fmm1 fmm2].
-        rewrite gmultiset_disj_union_left_id.
-        rewrite gmultiset_disj_union_left_id.
-        rewrite gmultiset_disj_union_left_id in fmm2.
-        rewrite multiplicity_disj_union in fmm1.
-        rewrite multiplicity_disj_union in fmm1.
-        rewrite not_elem_of_difference in m_in.
-        have h : Decision (m ∈ sa) by solve_decision. destruct h as [h|n].
-        + destruct m_in as [m_not_in_sa|mk].
-          * exfalso. apply m_not_in_sa. apply h.
-          * rewrite multiplicity_disj_union in fmm1.
-            have fmm1i := fmm1 h.
-            rewrite elem_of_singleton in mk. subst m. rewrite multiplicity_singleton in fmm1i.
-              rewrite multiplicity_empty in fmm1i. lia.
-        + have fmm2i := fmm2 n.
-          rewrite multiplicity_disj_union in fmm2i.
-          rewrite multiplicity_disj_union in fmm2i. lia.
-Qed.
+    intro a_not_in_b.
+    have X1 := X (elements (Elements := gset_elements) a).
+    assert (list_to_set (elements a) ⊈ b) as Y. { set_solver. }
+    have Z := X1 Y. destruct Z as [u [Z1 Z2]]. exists u. split; trivial.
+    rewrite list_to_set_elements in Z1. trivial.
+  Qed.
 
-Lemma bigSepS_alive_equiv_own a
-  (ne_emp: a ≠ ∅)
-    : ([∗ set] k ∈ a, Alive k) ⊣⊢ own γlt (LtOk None (list_to_set_disj (elements a)) ∅).
-Proof.
-  induction a as [|x T ? IH] using set_ind_L. 
-  - contradiction.
-  - have h : Decision (T = ∅) by solve_decision. destruct h as [h|n]; trivial.
-    + subst T. rewrite big_sepS_union; last by set_solver.
-      rewrite big_sepS_empty. rewrite big_sepS_singleton. unfold Alive, alive.
-      rewrite union_empty_r. rewrite elements_singleton. unfold list_to_set_disj.
-      rewrite bi.sep_emp. rewrite gmultiset_disj_union_right_id. trivial.
-    + rewrite big_sepS_union; last by set_solver.
-      rewrite (IH n). rewrite big_sepS_singleton. unfold Alive, alive.
-        rewrite <- own_op.
-        f_equiv.
-        unfold "⋅", cmra_op, ltR, lt_op. f_equiv; last by set_solver.
-        rewrite elements_union_singleton; trivial.
-Qed.
+  (*** Lifetime logic ***)
 
-Lemma lt_ok_none_left o a1 d1 a2 d2
-    : LtOk None a1 d1 ⋅ LtOk o a2 d2 = LtOk o (a1 ⊎ a2) (d1 ∪ d2).
-Proof.
-  destruct o as [o|]; trivial.
-Qed.
+  (* end hide *)
+  Definition NLLFT := nroot .@ "leaf-lifetime".
 
-Lemma mult_list_to_set_disj_not_in (a: gset nat) (x: nat)
-  (not_in: x ∉ a) : multiplicity x (list_to_set_disj (elements a)) = 0.
-Proof.
- induction a as [|y b ? IH] using set_ind_L. 
- - trivial.
- - rewrite elements_union_singleton; trivial. rewrite list_to_set_disj_cons.
-    rewrite multiplicity_disj_union. rewrite IH; last by set_solver.
-    assert (x ≠ y) by set_solver. rewrite multiplicity_singleton_ne; trivial.
-Qed.
-
-Lemma mult_list_to_set_disj_in (a: gset nat) (x: nat)
-  (is_in: x ∈ a) : multiplicity x (list_to_set_disj (elements a)) = 1.
-Proof.
- induction a as [|y b ? IH] using set_ind_L. 
- - rewrite elem_of_empty in is_in. contradiction.
- - rewrite elements_union_singleton; trivial. rewrite list_to_set_disj_cons.
-    rewrite multiplicity_disj_union.
-    rewrite elem_of_union in is_in. destruct is_in as [ix|ib].
-    + rewrite elem_of_singleton in ix. subst x. rewrite mult_list_to_set_disj_not_in; trivial.
-        rewrite multiplicity_singleton. trivial.
-    + rewrite (IH ib). rewrite multiplicity_singleton_ne; trivial. intro x_eq_y.
-        subst x. contradiction.
-Qed.
-
-Lemma multiplicity_le o1 a1 d1 o2 a2 d2 x
-  : LtOk o1 a1 d1 ≼ LtOk o2 a2 d2 → multiplicity x a1 ≤ multiplicity x a2.
-Proof.
-  intro incl. destruct incl as [t incl]. destruct t as [o3 a3 d3|].
-  - assert (a2 = a1 ⊎ a3) as X.
-      + unfold "⋅", lt_op in incl. destruct o1; destruct o3.
-        * inversion incl. * inversion incl; trivial. * inversion incl; trivial.
-        * inversion incl; trivial.
-      + subst a2. rewrite multiplicity_disj_union. lia.
-  - unfold "⋅", lt_op in incl. destruct o1; inversion incl.
-Qed.
-
-Lemma own_and_alive (a1 a2 : gset nat)
-  : own γlt (LtOk None (list_to_set_disj (elements a1)) ∅)
-    ∧ own γlt (LtOk None (list_to_set_disj (elements a2)) ∅)
-    ⊢ own γlt (LtOk None (list_to_set_disj (elements (a1 ∪ a2))) ∅).
-Proof.
-  iIntros "x".
-  iDestruct (and_own_discrete_ucmra_specific with "x") as "y"; last by iFrame "y".
-  intros w valw incl1 incl2.
-  destruct w as [o a d|].
-  - exists (LtOk o (a ∖ (list_to_set_disj (elements (a1 ∪ a2)))) d).
-    rewrite lt_ok_none_left. f_equiv.
-    + rewrite gmultiset_eq. intros x.
-        rewrite multiplicity_disj_union.
-        rewrite multiplicity_difference.
-        enough ((multiplicity x a ≥ multiplicity x (list_to_set_disj (elements (a1 ∪ a2))))).
-        { lia. }
-        have t1 := multiplicity_le _ _ _ _ _ _ x incl1.
-        have t2 := multiplicity_le _ _ _ _ _ _ x incl2.
-        have h : Decision (x ∈ a1) by solve_decision. destruct h as [h1|n1]; trivial.
-          *  rewrite mult_list_to_set_disj_in in t1; trivial.
-             rewrite mult_list_to_set_disj_in; last by set_solver.
-             lia.
-        * have q : Decision (x ∈ a2) by solve_decision. destruct q as [h2|n2]; trivial.
-          -- rewrite mult_list_to_set_disj_in in t2; trivial.
-             rewrite mult_list_to_set_disj_in; last by set_solver.
-             lia.
-          -- rewrite mult_list_to_set_disj_not_in; last by set_solver.
-             lia.
-    + set_solver.
-  - unfold "✓", cmra_valid, ucmra_cmraR, ucmra_valid, ltUR, lt_valid in valw.
-    destruct valw as [b valw].
-    replace (LtFail ⋅ b) with LtFail in valw. { contradiction. }
-    destruct b; trivial.
-Qed.
-
-Lemma alive_and_bigSepS (a1 a2 : gset nat)
-  : ([∗ set] k ∈ a1, Alive k) ∧ ([∗ set] k ∈ a2, Alive k)
-    ⊢ [∗ set] k ∈ a1 ∪ a2, Alive k.
-Proof.
-  have h: Decision (a1 = ∅) by solve_decision. destruct h as [h1|n1].
-  { subst a1. rewrite big_sepS_empty. rewrite bi.emp_and.
-      rewrite big_sepS_union; last by set_solver.
-      rewrite big_sepS_empty. rewrite bi.emp_sep. trivial. }
-  have h: Decision (a2 = ∅) by solve_decision. destruct h as [h2|n2].
-  { subst a2. rewrite big_sepS_empty. rewrite bi.and_emp.
-      rewrite big_sepS_union; last by set_solver.
-      rewrite big_sepS_empty. rewrite bi.sep_emp. trivial. }
-  rewrite bigSepS_alive_equiv_own; trivial.
-  rewrite bigSepS_alive_equiv_own; trivial.
-  rewrite bigSepS_alive_equiv_own; last by set_solver.
-  apply own_and_alive.
-Qed.
-        
-Local Instance pers_dead k : Persistent (Dead k).
-Proof.
-  apply own_core_persistent. unfold CoreId. trivial.
-Qed.
-
-Lemma LtState_entails_Dead k sa sd : (k ∈ sd) → LtState sa sd ⊢ Dead k.
-Proof.
-  intros ksd.
-  unfold LtState.
-  replace (lt_state sa sd) with (lt_state sa sd ⋅ dead k).
-  { rewrite own_op. iIntros "[A B]". iFrame "B". }
-  unfold dead, lt_state, "⋅", lt_op. f_equal. set_solver.
-Qed.
-
-Lemma LtState_disjoint sa sd : LtState sa sd ⊢ ⌜ sa ∩ sd = ∅ ⌝.
-Proof.
-  iIntros "T". iDestruct (own_valid with "T") as "%val". iPureIntro.
-  destruct val as [t lts].
-  destruct t as [[o|] a d|].
-  - inversion lts.
-  - simpl in lts. intuition.
-  - inversion lts.
-Qed.
-
-Definition Cancel (γ: gname) : iProp Σ := own γ (Excl ()).
-Lemma new_cancel : ⊢ |==> ∃ γ , Cancel γ.
-Proof.
-  iIntros. iDestruct (own_alloc (Excl ())) as "H"; first done. unfold Cancel. iFrame "H".
-Qed.
-Local Lemma cancel_cancel_false (γc : gname) : Cancel γc ∗ Cancel γc ⊢ False.
-Proof.
-  iIntros "X". unfold Cancel. rewrite <- own_op.
-  iDestruct (own_valid with "X") as "%J". contradiction.
-Qed.
-
-Local Lemma not_subset_eq_get (a b : gset nat) : (a ⊈ b) → ∃ k , k ∈ a ∧ k ∉ b.
-Proof.
-  assert (∀ r , list_to_set r ⊈ b → ∃ u: nat , u ∈ ((list_to_set r) : gset nat) ∧ u ∉ b) as X.
-  { intro r. induction r as [|a0 r IHr].
-    - intros emp. rewrite list_to_set_nil in emp. set_solver.
-    - intros not_in. rewrite list_to_set_cons in not_in.
-      destruct (decide (a0 ∈ b)); trivial.
-      + assert (list_to_set r ⊈ b) as K by set_solver.
-        have IHr2 := IHr K. destruct IHr2 as [u IHr2]. exists u. set_solver.
-      + exists a0. intuition. rewrite list_to_set_cons. set_solver.
-  }
-  intro a_not_in_b.
-  have X1 := X (elements (Elements := gset_elements) a).
-  assert (list_to_set (elements a) ⊈ b) as Y. { set_solver. }
-  have Z := X1 Y. destruct Z as [u [Z1 Z2]]. exists u. split; trivial.
-  rewrite list_to_set_elements in Z1. trivial.
-Qed.
-
-(* end hide *)
-
-(*** Lifetime logic ***)
-
-Definition NLLFT := nroot .@ "leaf-lifetime".
-
-Definition Lifetime := gset nat.
-
-Global Instance llft_intersect : Meet Lifetime := λ κ1 κ2, κ1 ∪ κ2.
-Definition llft_empty : Lifetime := ∅.
-
-Definition llft_alive (κ : Lifetime) : iProp Σ := [∗ set] k ∈ κ , Alive k.
-Definition llft_dead (κ : Lifetime) : iProp Σ := ∃ k , ⌜ k ∈ κ ⌝ ∗ Dead k.
-
-Definition llft_ctx :=
-  (True &&{↑NLLFT}&&> ∃ sa sd , LtState sa sd ∗ llft_alive sa).
-
-Definition llft_incl (κ1 κ2 : Lifetime) : iProp Σ :=
-    llft_alive κ1 &&{↑NLLFT}&&> llft_alive κ2.
-    
-Notation "@[ κ ]" := (llft_alive κ) (format "@[ κ ]") : bi_scope.
-Notation "@[† κ ]" := (llft_dead κ) (format "@[† κ ]") : bi_scope.
-Infix "⊑" := llft_incl (at level 70) : bi_scope.
-
-Global Instance pers_llft_ctx : Persistent llft_ctx.
-Proof. typeclasses eauto. Qed.
+  (** A Lifetime κ is defined as a [gset nat]. Though this should technically be
+  an implementation detail, this makes it easy to export the basic properties of [Lifetime]
+  (EqDecidable, Countable) and [⊓] (associativity, commutativity). *)
   
-Global Instance pers_llft_dead κ : Persistent (@[† κ ]).
-Proof. typeclasses eauto. Qed.
+  Definition Lifetime := gset nat.
 
-Global Instance timeless_llft_alive κ : Timeless (@[ κ ]).
-Proof. typeclasses eauto. Qed.
+  Global Instance llft_intersect : Meet Lifetime := λ κ1 κ2, κ1 ∪ κ2.
+  Definition llft_empty : Lifetime := ∅.
+  (* begin hide *)
 
-Global Instance timeless_llft_dead κ : Timeless (@[† κ ]).
-Proof. typeclasses eauto. Qed.
+  Local Definition llft_alive_def (κ : Lifetime) : iProp Σ := [∗ set] k ∈ κ , Alive k.
+  Local Definition llft_dead_def (κ : Lifetime) : iProp Σ := ∃ k , ⌜ k ∈ κ ⌝ ∗ Dead k.
+
+  Local Definition llft_ctx_def :=
+    (True &&{↑NLLFT}&&> ∃ sa sd , LtState sa sd ∗ llft_alive_def sa).
+
+  Local Definition llft_alive_aux : seal (@llft_alive_def). Proof. by eexists. Qed.
+  Local Definition llft_dead_aux : seal (@llft_dead_def). Proof. by eexists. Qed.
+  Local Definition llft_ctx_aux : seal (@llft_ctx_def). Proof. by eexists. Qed.
+
+  (* end hide *)
   
-Lemma llftl_not_own_end κ : @[ κ ] ∗ @[† κ ] ⊢ False.
-Proof.
-  iIntros "[A D]". iDestruct "D" as (k) "[%kk D]".
-  iDestruct ((big_sepS_delete _ _ k) with "A") as "[A _]". { trivial. }
-  iApply (lt_alive_dead_false k). iSplit; iFrame.
-Qed.
+  (** Definitions of the lifetime tokens. Note that these aren't fractional since you
+  use Leaf concepts instead. *)
+  
+  Definition llft_alive (κ : Lifetime) : iProp Σ. exact (llft_alive_aux.(unseal) κ). Defined.
+  Definition llft_dead (κ : Lifetime) : iProp Σ. exact (llft_dead_aux.(unseal) κ). Defined.
+  Definition llft_ctx : iProp Σ. exact (llft_ctx_aux.(unseal)). Defined.
+  (* begin hide *)
 
-Lemma llftl_not_own_end_and κ : @[ κ ] ∧ @[† κ ] ⊢ False.
-Proof.
-  iIntros "AD". unfold llft_dead. rewrite bi.and_exist_l. iDestruct "AD" as (k) "AD".
-  iApply (lt_alive_dead_false k).
-  iAssert (⌜k ∈ κ⌝)%I as "%kk". { iDestruct "AD" as "[_ [D _]]".  iFrame. }
-  iSplit; iFrame.
-  { iDestruct "AD" as "[A _]".
-    iDestruct ((big_sepS_delete _ _ k) with "A") as "[A _]". { trivial. } iFrame. }
-  { iDestruct "AD" as "[_ [_ D]]". iFrame. }
-Qed.
+  Local Definition llft_alive_unseal :
+      @llft_alive = @llft_alive_def := llft_alive_aux.(seal_eq).
+  Local Definition llft_dead_unseal :
+      @llft_dead = @llft_dead_def := llft_dead_aux.(seal_eq).
+  Local Definition llft_ctx_unseal :
+      @llft_ctx = @llft_ctx_def := llft_ctx_aux.(seal_eq).
 
-Lemma llftl_begin :
-    llft_ctx ⊢ |={↑NLLFT}=> ∃ κ, @[ κ ] ∗ (@[ κ ] ={↑NLLFT}=∗ @[† κ ]).
-Proof.
-    iIntros "#ctx".  unfold llft_ctx.
-    iDestruct (guards_open (True)%I _ (↑NLLFT) (↑NLLFT) with "[ctx]") as "J". { set_solver. }
-    { iFrame "ctx". }
-    iMod "J" as "[J back]". iDestruct "J" as (sa sd) "[State Alive]".
-    
-    assert (∃ k , k ∉ (sa ∪ sd)) as Fres. { exists (fresh (sa ∪ sd)). apply is_fresh. }
-    destruct Fres as [k Fres].
-    iMod (new_lt k sa sd with "[State]") as "T".
-    { set_solver. } { set_solver. } { iFrame. }
-    iDestruct "T" as "[State [A1 A2]]".
-    iMod ("back" with "[Alive State A1]").
-    { iExists (sa ∪ {[k]}). iExists sd. iFrame.
-      unfold llft_alive.
-      replace ((sa ∪ {[k]})) with (({[k]} ∪ sa)).
-      { rewrite big_sepS_insert. { iFrame. } set_solver. } set_solver.
-    }
+  Local Ltac unseal := rewrite
+    ?llft_alive_unseal /llft_alive_def
+    ?llft_dead_unseal /llft_dead_def
+    ?llft_ctx_unseal /llft_ctx_def.
+
+  (* end hide *)
+
+  Notation "@[ κ ]" := (llft_alive κ) (format "@[ κ ]") : bi_scope.
+  Notation "[† κ ]" := (llft_dead κ) (format "[† κ ]") : bi_scope.
+  
+  (** Lifetime inclusion is, by definition, a guard proposition. This provides us with
+  an analogue of RustBelt's "dynamic lifetime inclusion": to derive new lifetime inclusions
+  we can use Leaf to derive new guard propositions. *)
+  
+  Definition llft_incl (κ1 κ2 : Lifetime) : iProp Σ :=
+      @[ κ1 ] &&{↑NLLFT}&&> @[ κ2 ].
+  
+  Infix "⊑" := llft_incl (at level 70) : bi_scope.
+  
+  (** The lifetime logic *)
+
+  Global Instance pers_llft_ctx : Persistent llft_ctx.
+  Proof. unseal. typeclasses eauto. Qed.
+
+  Global Instance pers_llft_dead κ : Persistent ([† κ ]).
+  Proof. unseal. typeclasses eauto. Qed.
+
+  Global Instance timeless_llft_alive κ : Timeless (@[ κ ]).
+  Proof. unseal. typeclasses eauto. Qed.
+
+  Global Instance timeless_llft_dead κ : Timeless ([† κ ]).
+  Proof. unseal. typeclasses eauto. Qed.
+
+  Lemma llftl_not_own_end κ : @[ κ ] ∗ [† κ ] ⊢ False.
+  Proof.
+    unseal. iIntros "[A D]". iDestruct "D" as (k) "[%kk D]".
+    iDestruct ((big_sepS_delete _ _ k) with "A") as "[A _]". { trivial. }
+    iApply (lt_alive_dead_false k). iSplit; iFrame.
+  Qed.
+
+  Lemma llftl_not_own_end_and κ : @[ κ ] ∧ [† κ ] ⊢ False.
+  Proof.
+    unseal. iIntros "AD". unfold llft_dead. rewrite bi.and_exist_l. iDestruct "AD" as (k) "AD".
+    iApply (lt_alive_dead_false k).
+    iAssert (⌜k ∈ κ⌝)%I as "%kk". { iDestruct "AD" as "[_ [D _]]".  iFrame. }
+    iSplit; iFrame.
+    { iDestruct "AD" as "[A _]".
+      iDestruct ((big_sepS_delete _ _ k) with "A") as "[A _]". { trivial. } iFrame. }
+    { iDestruct "AD" as "[_ [_ D]]". iFrame. }
+  Qed.
+
+  Lemma llftl_begin :
+      llft_ctx ⊢ |={↑NLLFT}=> ∃ κ, @[ κ ] ∗ (@[ κ ] ={↑NLLFT}=∗ [† κ ]).
+  Proof.
+      unseal. iIntros "#ctx".  unfold llft_ctx.
+      iDestruct (guards_open (True)%I _ (↑NLLFT) (↑NLLFT) with "[ctx]") as "J". { set_solver. }
+      { iFrame "ctx". }
+      iMod "J" as "[J back]". iDestruct "J" as (sa sd) "[State Alive]".
+
+      assert (∃ k , k ∉ (sa ∪ sd)) as Fres. { exists (fresh (sa ∪ sd)). apply is_fresh. }
+      destruct Fres as [k Fres].
+      iMod (new_lt k sa sd with "[State]") as "T".
+      { set_solver. } { set_solver. } { iFrame. }
+      iDestruct "T" as "[State [A1 A2]]".
+      iMod ("back" with "[Alive State A1]").
+      { iExists (sa ∪ {[k]}). iExists sd. iFrame.
+        unfold llft_alive.
+        replace ((sa ∪ {[k]})) with (({[k]} ∪ sa)).
+        { unseal. rewrite big_sepS_insert. { iFrame. } set_solver. } set_solver.
+      }
+      iModIntro.
+      iExists ({[ k ]}). unfold llft_alive. 
+      rewrite big_sepS_singleton. iFrame "A2".
+      iIntros "token".
+
+      (* ending the lifetime *)
+      iDestruct (guards_open (True)%I _ (↑NLLFT) (↑NLLFT) with "[ctx]") as "J". { set_solver. }
+      { iFrame "ctx". }
+      iMod "J" as "[J back]". iDestruct "J" as (sa1 sd1) "[State Alive]".
+      iAssert (⌜k ∈ sa1⌝)%I as "%k_sa1".
+      { iApply (lt_state_alive k sa1 sd1). iSplit. { iFrame "State". } iFrame "token". }
+      unseal. rewrite (big_sepS_delete _ sa1 k); trivial.
+      iDestruct "Alive" as "[token2 Alive]".
+      iMod (kill_lt k sa1 sd1 with "[State token token2]") as "[State dead]". { iFrame. }
+      iMod ("back" with "[State Alive]") as "X".
+      { iExists (sa1 ∖ {[k]}). iExists (sd1 ∪ {[k]}). iFrame. }
+      iModIntro. unfold llft_dead. iExists k. iFrame "dead". iPureIntro. set_solver.
+  Qed.
+
+  Lemma llftl_borrow_shared κ (P : iProp Σ) :
+      ▷ P ={↑NLLFT}=∗ (@[ κ ] &&{↑NLLFT}&&> ▷ P) ∗ ([† κ ] ={↑NLLFT}=∗ ▷ P).
+  Proof.
+    iIntros "P".
+    iMod new_cancel as (γc) "c1".
+    iMod (inv_alloc_with_guard (NLLFT) (↑NLLFT) ((P ∨ (llft_dead κ ∗ Cancel γc))) with "[P]") as "[#Tinv #Tguard]".
+    { iNext. iLeft. iFrame "P". }
     iModIntro.
-    iExists ({[ k ]}). unfold llft_alive. 
-    rewrite big_sepS_singleton. iFrame "A2".
-    iIntros "token".
-    
-    (* ending the lifetime *)
-    iDestruct (guards_open (True)%I _ (↑NLLFT) (↑NLLFT) with "[ctx]") as "J". { set_solver. }
-    { iFrame "ctx". }
-    iMod "J" as "[J back]". iDestruct "J" as (sa1 sd1) "[State Alive]".
-    iAssert (⌜k ∈ sa1⌝)%I as "%k_sa1".
-    { iApply (lt_state_alive k sa1 sd1). iSplit. { iFrame "State". } iFrame "token". }
-    rewrite (big_sepS_delete _ sa1 k); trivial.
-    iDestruct "Alive" as "[token2 Alive]".
-    iMod (kill_lt k sa1 sd1 with "[State token token2]") as "[State dead]". { iFrame. }
-    iMod ("back" with "[State Alive]") as "X".
-    { iExists (sa1 ∖ {[k]}). iExists (sd1 ∪ {[k]}). iFrame. }
-    iModIntro. unfold llft_dead. iExists k. iFrame "dead". iPureIntro. set_solver.
-Qed.
-  
-Lemma llftl_borrow_shared κ (P : iProp Σ) :
-    ▷ P ={↑NLLFT}=∗ (@[ κ ] &&{↑NLLFT}&&> ▷ P) ∗ (@[† κ ] ={↑NLLFT}=∗ ▷ P).
-Proof.
-  iIntros "P".
-  iMod new_cancel as (γc) "c1".
-  iMod (inv_alloc_with_guard (NLLFT) (↑NLLFT) ((P ∨ (llft_dead κ ∗ Cancel γc))) with "[P]") as "[#Tinv #Tguard]".
-  { iNext. iLeft. iFrame "P". }
-  iModIntro.
-  iSplit.
-  { 
-    iAssert (llft_alive κ &&{ ↑NLLFT ∪ ↑NLLFT }&&> ▷ P) as "H".
-    { iApply
-      (guards_or (llft_alive κ) (llft_alive κ) (llft_dead κ ∗ Cancel γc) (▷ P)).
-      { iIntros "t". iApply (llftl_not_own_end_and κ). iSplit.
-        { iDestruct "t" as "[t _]". iFrame "t". }
-        { iDestruct "t" as "[_ [t _]]". iFrame "t". }
-      }
-      iSplit. { iApply guards_refl. }
-      { setoid_replace (llft_dead κ ∗ Cancel γc ∨ ▷ P)%I
-          with (▷ P ∨ llft_dead κ ∗ Cancel γc)%I.
-        { iDestruct (guards_true (↑NLLFT) (llft_alive κ)) as "gt".
-          iDestruct (guards_transitive (↑NLLFT) (llft_alive κ)%I with "[gt Tguard]") as "J".
-          { iFrame "Tguard". iFrame "gt". }
-          rewrite bi.later_or.
-          iDestruct (guards_remove_later_or_r (llft_dead κ ∗ Cancel γc) (▷ P) (↑NLLFT)) as "X".
-          iDestruct (guards_transitive (↑NLLFT) (llft_alive κ)%I with "[J X]") as "R".
-          { iFrame "J". iFrame "X". }
-          iFrame "R".
+    iSplit.
+    { 
+      iAssert (llft_alive κ &&{ ↑NLLFT ∪ ↑NLLFT }&&> ▷ P) as "H".
+      { iApply
+        (guards_or (llft_alive κ) (llft_alive κ) (llft_dead κ ∗ Cancel γc) (▷ P)).
+        { iIntros "t". iApply (llftl_not_own_end_and κ). iSplit.
+          { iDestruct "t" as "[t _]". iFrame "t". }
+          { iDestruct "t" as "[_ [t _]]". iFrame "t". }
         }
-        rewrite bi.or_comm. trivial.
-      }
-    }
-    rewrite subseteq_union_1_L. { iFrame "H". } set_solver.
-  }
-  iIntros "deadk".
-  iDestruct (guards_open (True)%I (▷ (P ∨ llft_dead κ ∗ Cancel γc))%I (↑ NLLFT) (↑ NLLFT) with "[Tguard]") as "J". { set_solver. }
-  { iFrame "Tguard". }
-  iMod "J" as "[J K]". rewrite bi.later_or. iDestruct "J" as "[P|J]".
-  { iDestruct ("K" with "[deadk c1]") as "K". { iRight. iFrame. }
-      iMod "K" as "K". iModIntro. iFrame "P". }
-  iDestruct "J" as "[_ c2]". iMod "c2".
-  iDestruct (cancel_cancel_false γc with "[c1 c2]") as "J". { iFrame. } iExFalso. iFrame "J".
-Qed.
-
-Lemma llftl_incl_dead_implies_dead κ κ' :
-    ⊢ llft_ctx ∗ κ ⊑ κ' ∗ @[† κ' ] ={↑NLLFT}=∗ @[† κ ].
-Proof.
-  iIntros "[#ctx [#incl #dead]]".
-  
-  unfold llft_incl.
-  
-  leaf_hyp "incl" rhs to (False)%I as "G2".
-  {
-    leaf_by_sep. iIntros "a". iExFalso.
-    iApply (llftl_not_own_end κ'). iFrame. iFrame "dead".
-  }
-  unfold llft_ctx.
-  leaf_hyp "ctx" rhs to ((∃ sa sd : gset nat, ⌜ κ ⊆ sa ⌝ ∗ LtState sa sd ∗ llft_alive sa)
-      ∨ (∃ sa sd : gset nat, ⌜ ¬(κ ⊆ sa) ⌝ ∗ LtState sa sd ∗ llft_alive sa) )%I
-      as "ctx2".
-  {
-    leaf_by_sep. iIntros "T". iSplitL.
-      - iDestruct "T" as (sa sd) "state_alive".
-        have h : Decision (κ ⊆ sa) by solve_decision. destruct h as [h|n]; trivial.
-        + iLeft. iExists sa. iExists sd. iFrame. iPureIntro. trivial.
-        + iRight. iExists sa. iExists sd. iFrame. iPureIntro. trivial.
-      - iIntros "T". iDestruct "T" as "[T|T]".
-        + iDestruct "T" as (sa sd) "[_ T]". iExists sa. iExists sd. iFrame.
-        + iDestruct "T" as (sa sd) "[_ T]". iExists sa. iExists sd. iFrame.
-    }
-  
-    iAssert (True &&{ ↑NLLFT}&&> (∃ sa sd : gset nat, ⌜κ ⊈ sa⌝ ∗ LtState sa sd ∗ llft_alive sa)) as "G3".
-      { iApply guards_or_guards_false. iFrame "ctx2". 
-        leaf_goal rhs to (llft_alive κ). { iFrame "G2". }
-        leaf_by_sep.
-        { iIntros "T". 
-            iDestruct "T" as (sa sd) "[%ksa [state alive]]".
-              unfold llft_alive.
-              replace sa with (κ ∪ (sa ∖ κ)) at 2.
-              { setoid_rewrite big_sepS_union.
-                { iDestruct "alive" as "[alive1 alive2]". iFrame "alive1".
-                  iIntros "rest".
-                  iExists sa. iExists sd. iFrame.
-                  iCombine "rest alive2" as "alive".
-                  setoid_rewrite <- big_sepS_union.
-                  { replace (κ ∪ sa ∖ κ) with sa. { iFrame. iPureIntro. trivial. }
-                  rewrite <- union_difference_L; trivial.
-               }
-               set_solver.
-            }
-            set_solver.
-        } rewrite <- union_difference_L; trivial.
-      }
-    }            
-    
-    leaf_open "G3" with "[]" as "[J back]". { set_solver. } { done. }
-     
-     iDestruct "J" as (sa sd) "[%k_sa [State alive]]".
-     have the_k := not_subset_eq_get κ sa k_sa. destruct the_k as [k [k_in k_not_in]].
-     have h : Decision (k ∈ sd) by solve_decision. destruct h as [h|n]; trivial.
-      - iDestruct (LtState_entails_Dead k sa sd with "State") as "#deadk"; trivial.
-        iMod ("back" with "[State alive]") as "true". { iExists sa. iExists sd. iFrame. iPureIntro; trivial. } iModIntro. unfold llft_dead. iExists k. iFrame "deadk". iPureIntro. apply k_in.
-      - (* weird technicality, if k was never made alive in the first place;
-          first create it, then immediately kill it *)
-        iMod (new_lt k sa sd with "State") as "[State [al1 al2]]"; trivial.
-        iMod (kill_lt k (sa ∪ {[ k ]}) sd with "[State al1 al2]") as "[State deadk]".
-          { iFrame. }
-        iMod ("back" with "[State alive]") as "J".
-        { iExists sa. iExists (sd ∪ {[k]}). iFrame.
-          replace (((sa ∪ {[k]}) ∖ {[k]})) with sa.
-          { iFrame. iPureIntro. trivial. } set_solver.
+        iSplit. { iApply guards_refl. }
+        { setoid_replace (llft_dead κ ∗ Cancel γc ∨ ▷ P)%I
+            with (▷ P ∨ llft_dead κ ∗ Cancel γc)%I.
+          { iDestruct (guards_true (↑NLLFT) (llft_alive κ)) as "gt".
+            iDestruct (guards_transitive (↑NLLFT) (llft_alive κ)%I with "[gt Tguard]") as "J".
+            { iFrame "Tguard". iFrame "gt". }
+            rewrite bi.later_or.
+            iDestruct (guards_remove_later_or_r (llft_dead κ ∗ Cancel γc) (▷ P) (↑NLLFT)) as "X".
+            iDestruct (guards_transitive (↑NLLFT) (llft_alive κ)%I with "[J X]") as "R".
+            { iFrame "J". iFrame "X". }
+            iFrame "R".
+          }
+          rewrite bi.or_comm. trivial.
         }
-        iModIntro. unfold llft_dead. iExists k. iFrame "deadk". iPureIntro; trivial.
-Qed.
+      }
+      rewrite subseteq_union_1_L. { iFrame "H". } set_solver.
+    }
+    iIntros "deadk".
+    iDestruct (guards_open (True)%I (▷ (P ∨ llft_dead κ ∗ Cancel γc))%I (↑ NLLFT) (↑ NLLFT) with "[Tguard]") as "J". { set_solver. }
+    { iFrame "Tguard". }
+    iMod "J" as "[J K]". rewrite bi.later_or. iDestruct "J" as "[P|J]".
+    { iDestruct ("K" with "[deadk c1]") as "K". { iRight. iFrame. }
+        iMod "K" as "K". iModIntro. iFrame "P". }
+    iDestruct "J" as "[_ c2]". iMod "c2".
+    iDestruct (cancel_cancel_false γc with "[c1 c2]") as "J". { iFrame. } iExFalso. iFrame "J".
+  Qed.
 
-Lemma llftl_incl_intersect κ κ' : ⊢ (κ ⊓ κ') ⊑ κ.
-Proof.
-  unfold llft_incl, llft_intersect, llft_alive.
-  leaf_by_sep. iIntros "Alive".
-  replace (κ ∪ κ') with (κ ∪ ((κ ∪ κ') ∖ κ)).
-  - rewrite big_sepS_union.
-    + iDestruct "Alive" as "[A1 A2]". iFrame "A1". iIntros "A3". iFrame.
-    + set_solver.
-  - symmetry. apply union_difference_L. set_solver.
-Qed.
+  Lemma llftl_incl_dead_implies_dead κ κ' :
+      ⊢ llft_ctx ∗ κ ⊑ κ' ∗ [† κ' ] ={↑NLLFT}=∗ [† κ ].
+  Proof.
+    unseal. iIntros "[#ctx [#incl #dead]]".
 
-Lemma llftl_incl_glb κ κ' κ'' :
-    κ ⊑ κ' ∗ κ ⊑ κ'' ⊢ κ ⊑ (κ' ⊓ κ'').
-Proof.
-  apply guards_and_point.
-   - unfold llft_alive. apply factoring_props.point_prop_big_sepS.
-      intros x xi. apply factoring_props.point_prop_own.
-   - unfold llft_alive. apply alive_and_bigSepS.
-Qed.
+    unfold llft_incl.
 
-Lemma llftl_tok_inter_l κ κ' :
-    @[ κ ⊓ κ' ] ⊢ @[ κ ].
-Proof.
-  unfold llft_intersect, llft_alive.
-  iIntros "Alive".
-  replace (κ ∪ κ') with (κ ∪ ((κ ∪ κ') ∖ κ)).
-  - rewrite big_sepS_union.
-    + iDestruct "Alive" as "[A1 A2]". iFrame "A1".
-    + set_solver.
-  - symmetry. apply union_difference_L. set_solver.
-Qed.
+    leaf_hyp "incl" rhs to (False)%I as "G2".
+    {
+      leaf_by_sep. iIntros "a". iExFalso.
+      iApply (llftl_not_own_end κ'). iFrame. unseal. iFrame "dead".
+    }
+    unfold llft_ctx.
+    leaf_hyp "ctx" rhs to ((∃ sa sd : gset nat, ⌜ κ ⊆ sa ⌝ ∗ LtState sa sd ∗ llft_alive sa)
+        ∨ (∃ sa sd : gset nat, ⌜ ¬(κ ⊆ sa) ⌝ ∗ LtState sa sd ∗ llft_alive sa) )%I
+        as "ctx2".
+    {
+      leaf_by_sep. iIntros "T". iSplitL.
+        - iDestruct "T" as (sa sd) "state_alive".
+          have h : Decision (κ ⊆ sa) by solve_decision. destruct h as [h|n]; trivial.
+          + unseal. iLeft. iExists sa. iExists sd. iFrame. iPureIntro. trivial.
+          + unseal. iRight. iExists sa. iExists sd. iFrame. iPureIntro. trivial.
+        - iIntros "T". iDestruct "T" as "[T|T]".
+          + iDestruct "T" as (sa sd) "[_ T]". iExists sa. iExists sd. unseal. iFrame.
+          + iDestruct "T" as (sa sd) "[_ T]". iExists sa. iExists sd. unseal. iFrame.
+      }
 
-Lemma llftl_tok_inter_r κ κ' :
-    @[ κ ⊓ κ' ] ⊢ @[ κ' ].
-Proof.
-  replace (κ ⊓ κ') with (κ' ⊓ κ).
-  - apply llftl_tok_inter_l. 
-  - unfold meet, llft_intersect. set_solver.
-Qed.
+      iAssert (True &&{ ↑NLLFT}&&> (∃ sa sd : gset nat, ⌜κ ⊈ sa⌝ ∗ LtState sa sd ∗ llft_alive sa)) as "G3".
+        { iApply guards_or_guards_false. iFrame "ctx2". 
+          leaf_goal rhs to (llft_alive κ). { iFrame "G2". }
+          leaf_by_sep.
+          { iIntros "T". 
+              iDestruct "T" as (sa sd) "[%ksa [state alive]]".
+                unseal. unfold llft_alive_def.
+                replace sa with (κ ∪ (sa ∖ κ)) at 2.
+                { setoid_rewrite big_sepS_union.
+                  { iDestruct "alive" as "[alive1 alive2]". iFrame "alive1".
+                    iIntros "rest".
+                    iExists sa. iExists sd. iFrame.
+                    iCombine "rest alive2" as "alive".
+                    setoid_rewrite <- big_sepS_union.
+                    { replace (κ ∪ sa ∖ κ) with sa. { iFrame. iPureIntro. trivial. }
+                    rewrite <- union_difference_L; trivial.
+                }
+                set_solver.
+              }
+              set_solver.
+          } rewrite <- union_difference_L; trivial.
+        }
+      }            
 
-Lemma llftl_tok_inter_and κ κ' :
-    @[ κ ⊓ κ' ] ⊣⊢ @[ κ ] ∧ @[ κ' ].
-Proof.
-  iIntros. iSplit.
-  - iIntros "t". iSplit.
-    + iApply llftl_tok_inter_l. iFrame "t".
-    + iApply llftl_tok_inter_r. iFrame "t".
- - unfold llft_alive. iIntros. iApply alive_and_bigSepS. iFrame.
-Qed.
+      leaf_open "G3" with "[]" as "[J back]". { set_solver. } { done. }
 
-Lemma llftl_end_inter κ κ' :
-    @[† κ ⊓ κ'] ⊣⊢ @[† κ ] ∨ @[† κ' ].
-Proof.
-  unfold llft_dead.
-  iIntros. iSplit.
-  - iIntros "t".  iDestruct "t" as (k) "[%kin t]".
-    unfold llft_intersect in kin. rewrite elem_of_union in kin. destruct kin as [h|h].
-    + iLeft. iExists k. iFrame "t". iPureIntro. trivial.
-    + iRight. iExists k. iFrame "t". iPureIntro. trivial.
-  - iIntros "t". iDestruct "t" as "[h|h]".
-    + iDestruct "h" as (k) "[%kin t]".
-      iExists k. iFrame "t". iPureIntro. unfold llft_intersect. set_solver.
-    + iDestruct "h" as (k) "[%kin t]".
-      iExists k. iFrame "t". iPureIntro. unfold llft_intersect. set_solver.
-Qed.
+      iDestruct "J" as (sa sd) "[%k_sa [State alive]]".
+      have the_k := not_subset_eq_get κ sa k_sa. destruct the_k as [k [k_in k_not_in]].
+      have h : Decision (k ∈ sd) by solve_decision. destruct h as [h|n]; trivial.
+        - iDestruct (LtState_entails_Dead k sa sd with "State") as "#deadk"; trivial.
+          iMod ("back" with "[State alive]") as "true". { iExists sa. iExists sd. iFrame. iPureIntro; trivial. } iModIntro. unfold llft_dead. iExists k. iFrame "deadk". iPureIntro. apply k_in.
+        - (* weird technicality, if k was never made alive in the first place;
+            first create it, then immediately kill it *)
+          iMod (new_lt k sa sd with "State") as "[State [al1 al2]]"; trivial.
+          iMod (kill_lt k (sa ∪ {[ k ]}) sd with "[State al1 al2]") as "[State deadk]".
+            { iFrame. }
+          iMod ("back" with "[State alive]") as "J".
+          { iExists sa. iExists (sd ∪ {[k]}). iFrame.
+            replace (((sa ∪ {[k]}) ∖ {[k]})) with sa.
+            { iFrame. iPureIntro. trivial. } set_solver.
+          }
+          iModIntro. unfold llft_dead. iExists k. iFrame "deadk". iPureIntro; trivial.
+  Qed.
 
-Lemma llftl_tok_unit :
-    ⊢ @[ llft_empty ].
-Proof.
-  unfold llft_alive, llft_empty. rewrite big_sepS_empty. iIntros. done.
-Qed.
+  Lemma llftl_incl_intersect κ κ' : ⊢ (κ ⊓ κ') ⊑ κ.
+  Proof.
+    leaf_by_sep. unseal. iIntros "Alive".
+    replace (κ ∪ κ') with (κ ∪ ((κ ∪ κ') ∖ κ)).
+    - rewrite big_sepS_union.
+      + iDestruct "Alive" as "[A1 A2]". iFrame "A1". iIntros "A3". iFrame.
+      + set_solver.
+    - symmetry. apply union_difference_L. set_solver.
+  Qed.
 
-Lemma llftl_end_unit :
-    @[† llft_empty ] ⊢ False.
-Proof.
-  unfold llft_dead, llft_empty. iIntros "t". iDestruct "t" as (k) "[%p t]".
-  rewrite elem_of_empty in p. contradiction.
-Qed.
+  Lemma llftl_incl_glb κ κ' κ'' :
+      κ ⊑ κ' ∗ κ ⊑ κ'' ⊢ κ ⊑ (κ' ⊓ κ'').
+  Proof.
+    apply guards_and_point.
+    - unseal. unfold llft_alive_def. apply factoring_props.point_prop_big_sepS.
+        intros x xi. apply factoring_props.point_prop_own.
+    - unseal. unfold llft_alive_def. apply alive_and_bigSepS.
+  Qed.
 
-End LtResource.
+  Lemma llftl_tok_inter_l κ κ' :
+      @[ κ ⊓ κ' ] ⊢ @[ κ ].
+  Proof.
+    iIntros "Alive".
+    replace (κ ∪ κ') with (κ ∪ ((κ ∪ κ') ∖ κ)).
+    - unseal. rewrite big_sepS_union.
+      + iDestruct "Alive" as "[A1 A2]". iFrame "A1".
+      + set_solver.
+    - symmetry. apply union_difference_L. set_solver.
+  Qed.
+
+  Lemma llftl_tok_inter_r κ κ' :
+      @[ κ ⊓ κ' ] ⊢ @[ κ' ].
+  Proof.
+    replace (κ ⊓ κ') with (κ' ⊓ κ).
+    - apply llftl_tok_inter_l. 
+    - unfold meet, llft_intersect. set_solver.
+  Qed.
+
+  Lemma llftl_tok_inter_and κ κ' :
+      @[ κ ⊓ κ' ] ⊣⊢ @[ κ ] ∧ @[ κ' ].
+  Proof.
+    iIntros. iSplit.
+    - iIntros "t". iSplit.
+      + iApply llftl_tok_inter_l. iFrame "t".
+      + iApply llftl_tok_inter_r. iFrame "t".
+  - unseal. iIntros. iApply alive_and_bigSepS. iFrame.
+  Qed.
+
+  Lemma llftl_end_inter κ κ' :
+      [† κ ⊓ κ'] ⊣⊢ [† κ ] ∨ [† κ' ].
+  Proof.
+    unseal. iIntros. iSplit.
+    - iIntros "t".  iDestruct "t" as (k) "[%kin t]".
+      unfold llft_intersect in kin. rewrite elem_of_union in kin. destruct kin as [h|h].
+      + iLeft. iExists k. iFrame "t". iPureIntro. trivial.
+      + iRight. iExists k. iFrame "t". iPureIntro. trivial.
+    - iIntros "t". iDestruct "t" as "[h|h]".
+      + iDestruct "h" as (k) "[%kin t]".
+        iExists k. iFrame "t". iPureIntro. unfold llft_intersect. set_solver.
+      + iDestruct "h" as (k) "[%kin t]".
+        iExists k. iFrame "t". iPureIntro. unfold llft_intersect. set_solver.
+  Qed.
+
+  Lemma llftl_tok_unit :
+      ⊢ @[ llft_empty ].
+  Proof.
+    unseal. unfold llft_empty. rewrite big_sepS_empty. iIntros. done.
+  Qed.
+
+  Lemma llftl_end_unit :
+      [† llft_empty ] ⊢ False.
+  Proof.
+    unseal. unfold llft_empty.
+    iIntros "t". iDestruct "t" as (k) "[%p t]".
+    rewrite elem_of_empty in p. contradiction.
+  Qed.
+
+End LlftLogic.
